Cleaned up formatting for trace arithmetic to match the rest of DY*

src/core/DY.Core.Trace.Arithmetic.Derived.fst
@@ -10,133 +10,157 @@ open DY.Core.Trace.Arithmetic
 
 /// Derived properties of trace arithmetic
 
-let trace_subtract_nil (#label_t:Type) (tr:trace_ label_t)
-  : Lemma
-    ((tr <--> empty_trace) == tr)
-    [SMTPat (tr <--> empty_trace)]
-  = trace_concat_subtract empty_trace tr
+val trace_subtract_empty_trace: #label_t:Type -> tr:trace_ label_t ->
+  Lemma ((tr <--> empty_trace) == tr)
+  [SMTPat (tr <--> empty_trace)]
+let trace_subtract_empty_trace tr = trace_concat_subtract empty_trace tr
 
-let trace_subtract_itself (#label_t:Type) (tr:trace_ label_t)
-  : Lemma
-    ((tr <--> tr) == empty_trace)
-    [SMTPat (tr <--> tr)]
-  = trace_concat_subtract tr empty_trace
+val trace_subtract_itself: #label_t:Type -> tr:trace_ label_t ->
+  Lemma ((tr <--> tr) == empty_trace)
+  [SMTPat (tr <--> tr)]
+let trace_subtract_itself tr = trace_concat_subtract tr empty_trace
 
-let trace_concat_snoc_right (#label_t:Type) (tr1 tr2:trace_ label_t) (e:trace_entry_ label_t)
-  : Lemma
-    (tr1 <++> (append_entry tr2 e) == append_entry (tr1 <++> tr2) e)
-  = trace_concat_assoc tr1 tr2 (append_entry empty_trace e)
+val trace_concat_append_entry:
+  #label_t:Type ->
+  tr1:trace_ label_t -> tr2:trace_ label_t ->
+  e:trace_entry_ label_t ->
+  Lemma (tr1 <++> (append_entry tr2 e) == append_entry (tr1 <++> tr2) e)
+let trace_concat_append_entry tr1 tr2 e =
+  trace_concat_assoc tr1 tr2 (append_entry empty_trace e)
 
-let trace_subtract_concat_left (#label_t:Type) (tr1 tr2 tr3:trace_ label_t)
-  : Lemma
-    (requires tr1 <$ tr2)
-    (ensures ((tr2 <--> tr1) <++> tr3) == ((tr2 <++> tr3) <--> tr1))
-  = trace_concat_assoc tr1 (tr2 <--> tr1) tr3
+val trace_subtract_concat_left:
+  #label_t:Type ->
+  tr1:trace_ label_t -> tr2:trace_ label_t -> tr3:trace_ label_t ->
+  Lemma
+  (requires tr1 <$ tr2)
+  (ensures ((tr2 <--> tr1) <++> tr3) == ((tr2 <++> tr3) <--> tr1))
+let trace_subtract_concat_left tr1 tr2 tr3 =
+  trace_concat_assoc tr1 (tr2 <--> tr1) tr3
 
-let trace_subtract_concat_slices (#label_t:Type) (tr1 tr2 tr3:trace_ label_t)
-  : Lemma
-    (requires tr1 <$ tr2 /\ tr2 <$ tr3)
-    (ensures (tr3 <--> tr1) == ((tr2 <--> tr1) <++> (tr3 <--> tr2)))
-    [SMTPat ((tr2 <--> tr1) <++> (tr3 <--> tr2))]
-  = trace_subtract_concat_left tr1 tr2 (tr3 <--> tr2);
-    trace_subtract_concat tr2 tr3
+val trace_subtract_concat_slices:
+  #label_t:Type ->
+  tr1:trace_ label_t -> tr2:trace_ label_t -> tr3:trace_ label_t ->
+  Lemma
+  (requires tr1 <$ tr2 /\ tr2 <$ tr3)
+  (ensures (tr3 <--> tr1) == ((tr2 <--> tr1) <++> (tr3 <--> tr2)))
+  [SMTPat ((tr2 <--> tr1) <++> (tr3 <--> tr2))]
+let trace_subtract_concat_slices tr1 tr2 tr3 =
+  trace_subtract_concat_left tr1 tr2 (tr3 <--> tr2);
+  trace_subtract_concat tr2 tr3
 
 
 /// Splitting a trace at a particular timestamp, getting the entry at that timestamp,
 /// along with the prefix before and suffix after that timestamp.
 /// Derived from trace subtraction.
 
-let trace_split (#label_t:Type) (tr:trace_ label_t) (ts:timestamp{ts `on_trace` tr})
-  : (trace_ label_t & trace_entry_ label_t & trace_ label_t)
-  = let tr1_e = prefix tr (ts + 1) in
-    (init tr1_e, last tr1_e, tr <--> tr1_e)
+val trace_split: #label_t:Type -> tr:trace_ label_t -> ts:timestamp{ts `on_trace` tr} ->
+  (trace_ label_t & trace_entry_ label_t & trace_ label_t)
+let trace_split tr ts =
+  let tr1_e = prefix tr (ts + 1) in
+  (init tr1_e, last tr1_e, tr <--> tr1_e)
 
 /// Properties of trace splitting
 
-let trace_split_trace_length (#label_t:Type) (tr:trace_ label_t) (ts:timestamp{ts `on_trace` tr})
-  : Lemma
-    (
-      let (tr1, e, tr2) = trace_split tr ts in
-      trace_length tr1 = ts /\ trace_length tr2 = (trace_length tr) - ts - 1
-    )
-    [SMTPat (trace_split tr ts)]
-  = ()
+val trace_split_trace_length: #label_t:Type -> tr:trace_ label_t -> ts:timestamp ->
+  Lemma
+  (requires ts `on_trace` tr)
+  (ensures (
+    let (tr1, e, tr2) = trace_split tr ts in
+    trace_length tr1 = ts /\ trace_length tr2 = (trace_length tr) - ts - 1
+  ))
+  [SMTPat (trace_split tr ts)]
+let trace_split_trace_length tr ts = ()
 
-let trace_split_get_entry (#label_t:Type) (tr:trace_ label_t) (ts:timestamp{ts `on_trace` tr}) (i:timestamp{i `on_trace` tr})
-  : Lemma
-    (
-      let (tr1, e, tr2) = trace_split tr ts in
-      get_entry_at tr i == (
-        if i < ts then get_entry_at tr1 i
-        else if i = ts then e
-        else get_entry_at tr2 (i - ts - 1)
-      )
+val trace_split_get_entry:
+  #label_t:Type -> tr:trace_ label_t ->
+  ts:timestamp -> i:timestamp ->
+  Lemma
+  (requires ts `on_trace` tr /\ i `on_trace` tr)
+  (ensures (
+    let (tr1, e, tr2) = trace_split tr ts in
+    get_entry_at tr i == (
+      if i < ts then get_entry_at tr1 i
+      else if i = ts then e
+      else get_entry_at tr2 (i - ts - 1)
     )
-  = let (tr1, e, tr2) = trace_split tr ts in
-    if i < ts then prefix_prefix_eq tr1 (prefix tr (ts + 1)) ts
-    else if i = ts then ()
-    else trace_subtract_get_entry (append_entry tr1 e) tr i
+  ))
+let trace_split_get_entry tr ts i =
+  let (tr1, e, tr2) = trace_split tr ts in
+  if i < ts then prefix_prefix_eq tr1 (prefix tr (ts + 1)) ts
+  else if i = ts then ()
+  else trace_subtract_get_entry (append_entry tr1 e) tr i
 
-let trace_split_fmap (#a #b:Type) (tr:trace_ a) (ts:timestamp{ts `on_trace` tr}) (f:a -> b)
-  : Lemma
-    (
+val trace_split_fmap: #a:Type -> #b:Type -> tr:trace_ a -> ts:timestamp -> f:(a -> b) ->
+  Lemma
+  (requires ts `on_trace` tr)
+  (ensures (
       let (tr1, e, tr2) = trace_split tr ts in
       let (tr1', e', tr2') = trace_split (fmap_trace f tr) ts in
       fmap_trace f tr1 == tr1' /\
       fmap_trace_entry f e == e' /\
       fmap_trace f tr2 == tr2'
-    )
-  = fmap_trace_prefix f tr (ts + 1);
-    trace_subtract_fmap_trace (prefix tr (ts + 1)) tr f
+  ))
+let trace_split_fmap tr ts f =
+  fmap_trace_prefix f tr (ts + 1);
+  trace_subtract_fmap_trace (prefix tr (ts + 1)) tr f
 
-let trace_split_matches_prefix (#label_t:Type) (tr:trace_ label_t) (ts:timestamp {ts `on_trace` tr})
-  : Lemma
-    (
-      let (tr1, e, _) = trace_split tr ts in
-      tr1 == prefix tr ts /\
-      append_entry tr1 e == prefix tr (ts + 1)
-    )
-  = let (tr1, e, _) = trace_split tr ts in
-    prefix_prefix_eq tr1 (prefix tr (ts + 1)) ts
+val trace_split_matches_prefix: #label_t:Type -> tr:trace_ label_t -> ts:timestamp ->
+  Lemma
+  (requires ts `on_trace` tr)
+  (ensures (
+    let (tr1, e, _) = trace_split tr ts in
+    tr1 == prefix tr ts /\
+    append_entry tr1 e == prefix tr (ts + 1)
+  ))
+let trace_split_matches_prefix tr ts =
+  let (tr1, e, _) = trace_split tr ts in
+  prefix_prefix_eq tr1 (prefix tr (ts + 1)) ts
 
-let trace_split_grows (#label_t:Type) (tr:trace_ label_t) (ts:timestamp{ts `on_trace` tr})
-  : Lemma
-    (
-      let (tr1, e, _) = trace_split tr ts in
-      tr1 <$ tr /\
-      (append_entry tr1 e) <$ tr
-    )
-  = trace_split_matches_prefix tr ts
+val trace_split_grows: #label_t:Type -> tr:trace_ label_t -> ts:timestamp ->
+  Lemma
+  (requires ts `on_trace` tr)
+  (ensures (
+    let (tr1, e, _) = trace_split tr ts in
+    tr1 <$ tr /\
+    (append_entry tr1 e) <$ tr
+  ))
+let trace_split_grows tr ts = trace_split_matches_prefix tr ts
 
 /// trace_split_at is a version of trace_split that allows us to more easily avoid
 /// dealing explicitly with timestamps in proofs, as we do not need to first use the
 /// fact that an entry exists on the trace to find the corresponding timestamp before
 /// splitting at that entry.
 
-let trace_split_at (#a:Type) (tr:trace_ a) (e:trace_entry_ a{entry_exists tr e})
-  : (trace_ a & (e':trace_entry_ a{trace_entry_equiv e e'}) & trace_ a)
-  = let idx = trace_find_first tr e in
-    let (tr1, e', tr2) = trace_split tr idx in
-    trace_split_get_entry tr idx idx;
-    (tr1, e', tr2)
+val trace_split_at:
+  #label_t:Type -> tr:trace_ label_t ->
+  e:trace_entry_ label_t{entry_exists tr e} ->
+  (trace_ label_t & (e':trace_entry_ label_t{trace_entry_equiv e e'}) & trace_ label_t)
+let trace_split_at tr e =
+  let idx = trace_find_first tr e in
+  let (tr1, e', tr2) = trace_split tr idx in
+  trace_split_get_entry tr idx idx;
+  (tr1, e', tr2)
 
 
 /// Properties relating split with concat and subtract
 
-let trace_split_concat (#label_t:Type) (tr:trace_ label_t) (ts:timestamp{ts `on_trace` tr})
-  : Lemma
-    (
-      let (tr1, e, tr2) = trace_split tr ts in
-       (append_entry tr1 e) <++> tr2 == tr
-    )
-  = trace_concat_subtract (prefix tr (ts + 1)) tr
+val trace_split_concat: #label_t:Type -> tr:trace_ label_t -> ts:timestamp ->
+  Lemma
+  (requires ts `on_trace` tr)
+  (ensures (
+    let (tr1, e, tr2) = trace_split tr ts in
+    (append_entry tr1 e) <++> tr2 == tr
+  ))
+let trace_split_concat tr ts = trace_concat_subtract (prefix tr (ts + 1)) tr
 
-let trace_subtract_matches_split (#label_t:Type) (tr1 tr2:trace_ label_t)
-  : Lemma
-    (requires tr1 <$ tr2 /\ is_not_empty tr1)
-    (ensures (
-      let (_, _, tl) = trace_split tr2 (trace_length tr1 - 1) in
-      tl == (tr2 <--> tr1)
-    ))
-  = prefix_prefix_eq tr1 tr2 (trace_length tr1)
+val trace_subtract_append_entry_matches_split:
+  #label_t:Type -> tr1:trace_ label_t -> tr2:trace_ label_t ->
+  Lemma
+  (requires tr1 <$ tr2 /\ is_not_empty tr1)
+  (ensures (
+    let (_, _, tl) = trace_split tr2 (trace_length tr1 - 1) in
+    tl == (tr2 <--> tr1)
+  ))
+let trace_subtract_append_entry_matches_split tr1 tr2 =
+  prefix_prefix_eq tr1 tr2 (trace_length tr1)
 
